Added request-response pair functions; Code clean up

src/request_response/DY.Example.RequestResponse.Protocol.Total.Proof.fst
@@ -1,10 +1,10 @@
-module DY.Example.SingleConfAuthMessage.Protocol.Total.Proof
+module DY.Example.RequestResponse.Protocol.Total.Proof
 
 open Comparse
 open DY.Core
 open DY.Lib
-open DY.Example.SingleConfAuthMessage.Protocol.Total
-open DY.Example.SingleConfAuthMessage.Protocol.Stateful
+open DY.Example.RequestResponse.Protocol.Total
+open DY.Example.RequestResponse.Protocol.Stateful
 
 #set-options "--fuel 0 --ifuel 0 --z3cliopt 'smt.qi.eager_threshold=100'"
 
@@ -15,12 +15,17 @@ instance crypto_usages_protocol = default_crypto_usages
 
 val pkenc_pred_list_protocol: list (string & pkenc_crypto_predicate)
 let pkenc_pred_list_protocol = [
-  pkenc_crypto_predicates_communication_layer_and_tag;
+  pkenc_crypto_predicates_communication_layer_and_tag
 ]
 
 val sign_pred_list_protocol: list (string & sign_crypto_predicate)
 let sign_pred_list_protocol = [
   sign_crypto_predicates_communication_layer_and_tag;
+]
+
+val aead_pred_list_protocol: list (string & aead_crypto_predicate)
+let aead_pred_list_protocol = [
+  aead_crypto_predicates_communication_layer_and_tag;
 ]
 
 #push-options "--ifuel 2 --fuel 0"
@@ -31,13 +36,15 @@ let crypto_predicates_protocol = {
   pkenc_pred = mk_pkenc_predicate pkenc_pred_list_protocol;
 
   sign_pred = mk_sign_predicate sign_pred_list_protocol;
+
+  aead_pred = mk_aead_predicate aead_pred_list_protocol;
 }
+#pop-options
 
 instance crypto_invariants_protocol: crypto_invariants = {
   usages = crypto_usages_protocol;
   preds = crypto_predicates_protocol;
 }
-#pop-options
 
 #push-options "--ifuel 0 --fuel 1"
 val pkenc_pred_has_all_pkenc_preds: 
@@ -49,7 +56,7 @@ val pkenc_pred_has_all_pkenc_preds:
     )
   )
 let pkenc_pred_has_all_pkenc_preds () =
-  assert_norm(List.Tot.no_repeats_p (List.Tot.map fst pkenc_pred_list_protocol));
+  assert_norm(List.Tot.no_repeats_p (List.Tot.map fst (pkenc_pred_list_protocol)));
   mk_pkenc_predicate_correct pkenc_pred_list_protocol;
   norm_spec [delta_only [`%pkenc_pred_list_protocol; `%for_allP]; iota; zeta] (for_allP has_pkenc_predicate pkenc_pred_list_protocol);
   ()
@@ -67,54 +74,64 @@ let sign_pred_has_all_sign_preds () =
   mk_sign_predicate_correct sign_pred_list_protocol;
   norm_spec [delta_only [`%sign_pred_list_protocol; `%for_allP]; iota; zeta] (for_allP has_sign_predicate sign_pred_list_protocol);
   ()
+
+val aead_pred_has_all_aead_preds:
+  unit ->
+  Lemma
+  (ensures
+    norm [delta_only [`%aead_pred_list_protocol; `%for_allP]; iota; zeta] (
+      for_allP has_aead_predicate aead_pred_list_protocol
+    )
+  )
+let aead_pred_has_all_aead_preds () =
+  assert_norm(List.Tot.no_repeats_p (List.Tot.map fst (aead_pred_list_protocol)));
+  mk_aead_predicate_correct aead_pred_list_protocol;
+  norm_spec [delta_only [`%aead_pred_list_protocol; `%for_allP]; iota; zeta] (for_allP has_aead_predicate aead_pred_list_protocol);
+  ()
 #pop-options
 
-val protocol_crypto_invariants_has_communication_layer_crypto_predicates: squash has_communication_layer_crypto_predicates
+val protocol_crypto_invariants_has_communication_layer_crypto_predicates: squash has_communication_layer_reqres_crypto_predicates
 let protocol_crypto_invariants_has_communication_layer_crypto_predicates =
   pkenc_pred_has_all_pkenc_preds ();
   sign_pred_has_all_sign_preds ();
+  aead_pred_has_all_aead_preds ();
   ()
-
 
 (*** Proofs ***)
 
 val compute_message_proof:
   tr:trace ->
-  sender:principal -> receiver:principal ->
-  secret:bytes ->
+  client:principal -> server:principal ->
+  nonce:bytes ->
   Lemma
   (requires
-    event_triggered tr sender (SenderSendMsg sender receiver secret) /\
-    bytes_invariant tr secret /\
-    is_knowable_by (join (principal_label sender) (principal_label receiver)) tr secret
+    is_knowable_by (join (principal_label client) (principal_label server)) tr nonce
   )
   (ensures
-    is_knowable_by (join (principal_label sender) (principal_label receiver)) tr (compute_message secret)
+    is_knowable_by (join (principal_label client) (principal_label server)) tr (compute_message client nonce)
   )
-let compute_message_proof tr sender receiver secret =
-  serialize_wf_lemma message (is_knowable_by (join (principal_label sender) (principal_label receiver)) tr) (Msg {secret;});
+let compute_message_proof tr client server nonce =
+  let req:request = { client; nonce } in
+  serialize_wf_lemma request (is_knowable_by (join (principal_label client) (principal_label server)) tr) req;
   ()
 
 val decode_message_proof:
   tr:trace ->
-  sender:principal -> receiver:principal ->
-  msg_bytes:bytes ->
+  server:principal ->
+  req_bytes:bytes -> req_label:label ->
   Lemma
   (requires
-    is_knowable_by (principal_label receiver) tr msg_bytes
+    is_knowable_by req_label tr req_bytes
   )
   (ensures (
-    match decode_message msg_bytes with
-    | Some msg -> (
-      is_knowable_by (principal_label receiver) tr msg.secret
-    )
+    match decode_message req_bytes with
     | None -> True
-  )
-  )
-let decode_message_proof tr sender receiver msg_bytes =
-  match decode_message msg_bytes with
-  | Some msg -> (
-      parse_wf_lemma message (is_knowable_by (principal_label receiver) tr) msg_bytes;
+    | Some {client=client'; nonce} -> is_knowable_by req_label tr nonce
+  ))
+let decode_message_proof tr server req_bytes req_label =
+  match decode_message req_bytes with
+  | None -> ()
+  | Some {client; nonce} -> (    
+    parse_wf_lemma request (is_knowable_by req_label tr) req_bytes;
     ()
   )
-  | None -> ()
