src/request_response/DY.Example.RequestResponse.Debug.fst
@@ -1,0 +1,32 @@
+module DY.Example.RequestResponse.Debug
+
+open DY.Core
+open DY.Lib
+
+open DY.Example.RequestResponse.Protocol.Stateful
+
+let debug () : traceful (option unit) =
+  let _ = IO.debug_print_string "************* Trace *************\n" in
+  (*** Initialize protocol run ***)
+  let client = "client" in
+  let server = "server" in
+
+  let*? client_comm_keys_sess_ids, server_comm_keys_sess_ids = initialize_communication client server in
+
+  let*? (sid, msg_id) = client_send_request client_comm_keys_sess_ids client server in
+
+  let*? msg_id = server_receive_request_send_response server_comm_keys_sess_ids server msg_id in
+
+  client_receive_response client_comm_keys_sess_ids client sid msg_id;*?
+
+  let* tr = get_trace in
+  let _ = IO.debug_print_string (
+      trace_to_string default_trace_to_string_printers tr
+    ) in
+  
+  return (Some ())
+
+//Run ``debug ()`` when the module loads
+#push-options "--warn_error -272"
+let _ = debug () Nil
+#pop-options
