src/request_response/DY.Example.RequestResponse.Protocol.Stateful.Proof.fst
@@ -1,0 +1,233 @@
+module DY.Example.RequestResponse.Protocol.Stateful.Proof
+
+open Comparse
+open DY.Core
+open DY.Lib
+
+open DY.Example.RequestResponse.Protocol.Total
+open DY.Example.RequestResponse.Protocol.Total.Proof
+open DY.Example.RequestResponse.Protocol.Stateful
+
+#set-options "--fuel 0 --ifuel 0 --z3cliopt 'smt.qi.eager_threshold=100'"
+
+(*** State Predicates ***)
+
+#push-options "--ifuel 3 --z3rlimit 20"
+let state_predicates_protocol: local_state_predicate protocol_state = {
+  pred = (fun tr prin sess_id st -> 
+    match st with
+    | ClientSendRequest {server; cmeta_data; nonce} -> (
+      let client = prin in
+      comm_meta_data_knowable tr client cmeta_data /\
+      is_secret (join (principal_label client) (principal_label server)) tr nonce
+    )
+    | ServerReceiveRequest {client; nonce} -> (
+      let server = prin in
+      is_knowable_by (join (principal_label client) (principal_label server)) tr nonce
+    )
+    | ClientReceiveResponse {server; cmeta_data; nonce} -> (
+      let client = prin in
+      comm_meta_data_knowable tr client cmeta_data /\
+      is_secret (join (principal_label client) (principal_label server)) tr nonce
+    )
+  );
+  pred_later = (fun tr1 tr2 prin sess_id state -> ());
+  pred_knowable = (fun tr prin sess_id state -> ());
+}
+#pop-options
+
+val protocol_state_tag: string
+let protocol_state_tag = "Protocol.State"
+
+let all_sessions = [
+  pki_tag_and_invariant;
+  private_keys_tag_and_invariant;
+  state_predicates_communication_layer_and_tag;
+  (|protocol_state_tag, local_state_predicate_to_local_bytes_state_predicate state_predicates_protocol|);
+]
+
+(*** Event Predicates ***)
+
+#push-options "--ifuel 2"
+val comm_layer_event_preds: comm_reqres_higher_layer_event_preds
+let comm_layer_event_preds = {
+  default_comm_reqres_higher_layer_event_preds with
+  send_request = (fun tr client server payload key_label ->
+    match decode_message payload with
+    | None -> False
+    | Some {client; nonce} -> is_secret (join (principal_label client) (principal_label server)) tr nonce
+  );
+  send_request_later = (fun tr1 tr2 client server payload key_label -> ())
+}
+#pop-options
+
+let all_events = event_predicate_communication_layer_reqres_and_tag comm_layer_event_preds
+
+(*** Combine all Invariants ***)
+
+/// Create the global trace invariants.
+
+let trace_invariants_protocol: trace_invariants = {
+  state_pred = mk_state_pred all_sessions;
+  event_pred = mk_event_pred all_events;
+}
+
+instance protocol_invariants_protocol: protocol_invariants = {
+  crypto_invs = crypto_invariants_protocol;
+  trace_invs = trace_invariants_protocol;
+}
+
+/// Lemmas that the global state predicate contains all the local ones
+
+val all_sessions_has_all_sessions: unit -> Lemma (norm [delta_only [`%all_sessions; `%for_allP]; iota; zeta] (for_allP has_local_bytes_state_predicate all_sessions))
+let all_sessions_has_all_sessions () =
+  assert_norm(List.Tot.no_repeats_p (List.Tot.map dfst (all_sessions)));
+  mk_state_pred_correct all_sessions;
+  norm_spec [delta_only [`%all_sessions; `%for_allP]; iota; zeta] (for_allP has_local_bytes_state_predicate all_sessions)
+
+val protocol_invariants_protocol_has_pki_invariant: squash has_pki_invariant
+let protocol_invariants_protocol_has_pki_invariant = all_sessions_has_all_sessions ()
+
+val protocol_invariants_protocol_has_private_keys_invariant: squash has_private_keys_invariant
+let protocol_invariants_protocol_has_private_keys_invariant = all_sessions_has_all_sessions ()
+
+val protocol_invariants_protocol_has_communication_layer_state_invariant: squash (has_local_state_predicate state_predicates_communication_layer)
+let protocol_invariants_protocol_has_communication_layer_state_invariant = all_sessions_has_all_sessions ()
+
+val protocol_invariants_protocol_has_protocol_state_invariant: squash (has_local_state_predicate state_predicates_protocol)
+let protocol_invariants_protocol_has_protocol_state_invariant = all_sessions_has_all_sessions ()
+
+/// Lemmas that the global event predicate contains all the local ones
+
+val all_events_has_all_events: unit -> Lemma (norm [delta_only [`%all_events; `%for_allP]; iota; zeta] (for_allP has_compiled_event_pred all_events))
+let all_events_has_all_events () =
+  assert_norm(List.Tot.no_repeats_p (List.Tot.map fst (all_events)));
+  mk_event_pred_correct all_events;
+  norm_spec [delta_only [`%all_events; `%for_allP]; iota; zeta] (for_allP has_compiled_event_pred all_events);
+  let dumb_lemma (x:prop) (y:prop): Lemma (requires x /\ x == y) (ensures y) = () in
+  dumb_lemma (for_allP has_compiled_event_pred all_events) (norm [delta_only [`%all_events; `%for_allP]; iota; zeta] (for_allP has_compiled_event_pred all_events))
+
+val protocol_invariants_has_communication_layer_event_invariants: squash (has_event_pred (event_predicate_communication_layer request_response_event_preconditions))
+let protocol_invariants_has_communication_layer_event_invariants = all_events_has_all_events ()
+
+#push-options "--fuel 1"
+val protocol_invariants_protocol_communication_layer_reqres_event_invariant: squash (has_event_pred (event_predicate_communication_layer_reqres comm_layer_event_preds))
+let protocol_invariants_protocol_communication_layer_reqres_event_invariant = all_events_has_all_events ()
+#pop-options
+
+(*** Proofs ***)
+
+#push-options "--z3rlimit 10"
+val client_send_request_proof:
+  tr:trace ->
+  comm_keys_ids:communication_keys_sess_ids ->
+  client:principal -> server:principal ->
+  Lemma
+  (requires
+    trace_invariant tr
+  )
+  (ensures (
+    let (_, tr_out) = client_send_request comm_keys_ids client server tr in
+    trace_invariant tr_out
+  ))
+  [SMTPat (trace_invariant tr); SMTPat (client_send_request comm_keys_ids client server tr)]
+let client_send_request_proof tr comm_keys_ids client server =
+  match client_send_request comm_keys_ids client server tr with
+  | (None, tr_out) -> (
+    let (nonce, tr) = mk_rand NoUsage (join (principal_label client) (principal_label server)) 32 tr in
+    compute_message_proof tr client server nonce;
+    let req_msg_bytes = compute_message client nonce in
+    send_request_proof tr comm_keys_ids comm_layer_event_preds client server req_msg_bytes;
+    ()
+  )
+  | (Some (sid, msg_id), tr_out) -> (
+    let (nonce, tr) = mk_rand NoUsage (join (principal_label client) (principal_label server)) 32 tr in
+    compute_message_proof tr client server nonce;
+    let req_msg_bytes = compute_message client nonce in
+    send_request_proof tr comm_keys_ids comm_layer_event_preds client server req_msg_bytes;
+    let (Some (req_bytes, cmeta_data), tr) = send_request comm_keys_ids client server req_msg_bytes tr in
+    let (sid, tr) = new_session_id client tr in
+    let ((), tr) = set_state client sid (ClientSendRequest { server; cmeta_data; nonce } <: protocol_state) tr in
+    assert(tr == tr_out);
+    assert(trace_invariant tr_out);
+    ()
+  )
+#pop-options
+
+#push-options "--ifuel 2 --z3rlimit 20"
+val server_receive_request_send_response_proof:
+  tr:trace ->
+  comm_keys_ids:communication_keys_sess_ids ->
+  server:principal ->
+  msg_id:timestamp ->
+  Lemma
+  (requires
+    trace_invariant tr
+  )
+  (ensures (
+    let (_, tr_out) = server_receive_request_send_response comm_keys_ids server msg_id tr in
+    trace_invariant tr_out
+  ))
+  [SMTPat (trace_invariant tr); SMTPat (server_receive_request_send_response comm_keys_ids server msg_id tr)]
+let server_receive_request_send_response_proof tr comm_keys_ids server msg_id =
+  receive_request_proof tr comm_keys_ids comm_layer_event_preds server msg_id;
+  match server_receive_request_send_response comm_keys_ids server msg_id tr with
+  | (None, tr_out) -> (
+    match receive_request comm_keys_ids server msg_id tr with
+    | (None, tr) -> ()
+    | (Some (req_bytes, cmeta_data), tr) -> (
+      decode_message_proof tr server req_bytes (get_response_label tr cmeta_data);
+
+      FStar.Classical.move_requires (parse_wf_lemma request (is_publishable tr)) req_bytes;
+      ()
+    )
+  )
+  | (Some msg_id', tr_out) -> (
+    let (Some (req_bytes, cmeta_data), tr) = receive_request comm_keys_ids server msg_id tr in
+    
+    decode_message_proof tr server req_bytes (get_response_label tr cmeta_data);
+    let Some req:option request = decode_message req_bytes in
+
+    assert(is_secret (join (principal_label req.client) (principal_label server)) tr req.nonce \/
+      is_publishable tr req_bytes);
+    FStar.Classical.move_requires (parse_wf_lemma request (is_publishable tr)) req_bytes;
+    assert(is_knowable_by (join (principal_label req.client) (principal_label server)) tr req.nonce);
+
+    let (sid, tr) = new_session_id server tr in
+    let ((), tr) = set_state server sid (ServerReceiveRequest { client=req.client; nonce=req.nonce } <: protocol_state) tr in
+    assert(trace_invariant tr);
+
+    send_response_proof tr comm_keys_ids comm_layer_event_preds server cmeta_data req.nonce;
+    let (Some msg_id, tr) = send_response comm_keys_ids server cmeta_data req.nonce tr in
+
+    assert(tr == tr_out);
+    assert(trace_invariant tr_out);
+    ()
+  )
+#pop-options
+
+val client_receive_response_proof:
+  tr:trace ->
+  comm_keys_ids:communication_keys_sess_ids ->
+  client:principal ->
+  sid:state_id -> msg_id:timestamp ->
+  Lemma
+  (requires
+    trace_invariant tr
+  )
+  (ensures (
+    let (_, tr_out) = client_receive_response comm_keys_ids client sid msg_id tr in
+    trace_invariant tr_out
+  ))
+  [SMTPat (trace_invariant tr); SMTPat (client_receive_response comm_keys_ids client sid msg_id tr)]
+let client_receive_response_proof tr comm_keys_ids client sid msg_id =
+  match get_state client sid tr with
+  | (None, tr) -> ()
+  | (Some state, tr) -> (
+    match state with
+    | ClientSendRequest {server; cmeta_data; nonce} ->(
+    receive_response_proof tr comm_keys_ids comm_layer_event_preds client cmeta_data msg_id;
+    ()
+    )
+    | _ -> ()
+  )  
