src/request_response/DY.Example.RequestResponse.Protocol.Stateful.fst
@@ -1,0 +1,83 @@
+module DY.Example.RequestResponse.Protocol.Stateful
+
+open Comparse
+open DY.Core
+open DY.Lib
+
+open DY.Example.RequestResponse.Protocol.Total
+
+[@@with_bytes bytes]
+type client_state = {
+  server: principal;
+  cmeta_data: comm_meta_data;
+  nonce: bytes;
+}
+
+%splice [ps_client_state] (gen_parser (`client_state))
+%splice [ps_client_state_is_well_formed] (gen_is_well_formed_lemma (`client_state))
+
+[@@with_bytes bytes]
+type server_state = {
+  client: principal;
+  nonce: bytes;
+}
+
+%splice [ps_server_state] (gen_parser (`server_state))
+%splice [ps_server_state_is_well_formed] (gen_is_well_formed_lemma (`server_state))
+
+[@@with_bytes bytes]
+type protocol_state =
+  | ClientSendRequest: client_state -> protocol_state
+  | ServerReceiveRequest: server_state -> protocol_state
+  | ClientReceiveResponse: client_state -> protocol_state
+
+
+%splice [ps_protocol_state] (gen_parser (`protocol_state))
+%splice [ps_protocol_state_is_well_formed] (gen_is_well_formed_lemma (`protocol_state))
+
+instance parseable_serializeable_bytes_protocol_state: parseable_serializeable bytes protocol_state
+  = mk_parseable_serializeable ps_protocol_state
+
+instance local_state_protocol_state: local_state protocol_state = {
+  tag = "Protocol.State";
+  format = parseable_serializeable_bytes_protocol_state;
+}
+
+(*** Protocol Functions ***)
+
+val client_send_request:
+  communication_keys_sess_ids ->
+  principal -> principal ->
+  traceful (option (state_id & timestamp))
+let client_send_request comm_keys_ids client server =
+  let* nonce = mk_rand NoUsage (join (principal_label client) (principal_label server)) 32 in
+  let payload = compute_message client nonce in
+  let*? (msg_id, cmeta_data) = send_request comm_keys_ids client server payload in
+  let* sid = new_session_id client in
+  set_state client sid (ClientSendRequest { server; cmeta_data; nonce } <: protocol_state);*
+  return (Some (sid, msg_id))
+
+val server_receive_request_send_response:
+  communication_keys_sess_ids ->
+  principal -> timestamp ->
+  traceful (option timestamp)
+let server_receive_request_send_response comm_keys_ids server msg_id =
+  let*? (req_bytes, req_meta_data) = receive_request comm_keys_ids server msg_id in
+  let*? req:request = return (decode_message req_bytes) in
+  let* sid = new_session_id server in
+  set_state server sid (ServerReceiveRequest { client=req.client; nonce=req.nonce } <: protocol_state);*
+  let*? msg_id = send_response comm_keys_ids server req_meta_data req.nonce in
+  return (Some msg_id)
+
+val client_receive_response:
+  communication_keys_sess_ids ->
+  principal -> state_id -> timestamp ->
+  traceful (option unit)
+let client_receive_response comm_keys_ids client sid msg_id =
+  let*? cstate = get_state client sid in
+  guard_tr (ClientSendRequest? cstate);*?
+  let ClientSendRequest { server; cmeta_data; nonce } = cstate in
+  let*? (res_bytes, _) = receive_response comm_keys_ids client cmeta_data msg_id in
+  guard_tr (res_bytes = nonce);*?
+  set_state client sid (ClientReceiveResponse { server; cmeta_data; nonce } <: protocol_state);*
+  return (Some ())
