src/request_response/DY.Example.RequestResponse.Protocol.Total.fst
@@ -1,0 +1,31 @@
+module DY.Example.RequestResponse.Protocol.Total
+
+open Comparse
+open DY.Core
+open DY.Lib
+
+(*
+  Client -> Server: enc{client, nonce}
+  Server -> Client: enc{nonce}
+*)
+
+[@@with_bytes bytes]
+type request = {
+  client: principal;
+  nonce: bytes;
+}
+
+%splice [ps_request] (gen_parser (`request))
+%splice [ps_request_is_well_formed] (gen_is_well_formed_lemma (`request))
+
+instance parseable_serializeable_bytes_request: parseable_serializeable bytes request
+  = mk_parseable_serializeable ps_request
+
+val compute_message: principal -> bytes -> bytes
+let compute_message client nonce =
+  let req = { client; nonce } in
+  serialize request req
+
+val decode_message: bytes -> option request
+let decode_message msg =
+  parse request msg
