Makefile
@@ -1,5 +1,5 @@
 DY_HOME ?= ../dolev-yao-star-extrinsic
 
-EXAMPLES = single_conf_message single_auth_message single_conf_and_auth_message
+EXAMPLES = single_conf_message single_auth_message single_conf_and_auth_message request_response
 EXAMPLE_DIRS = $(addprefix src/, $(EXAMPLES))
 include $(DY_HOME)/Makefile
